\section{Forward preservation lemma for rejection soundness}
\label{sec:rs2-proof}
\autoref{eq:rs2}

\begin{align*}
  &\forall(p:\Prog)(q,c,a:\Int)(s_0,s':\sigma)(v:\beta),\\
  &\sstep_p(q,c,s_0)=(a,s')\wedge\Reflects{v}{s_0}\\
  &\implies\exists v':\beta,\vstep_p(q,a,v)=\Some{v'}\wedge\Reflects{v'}{s'}
\end{align*}

The invariant $\Reflects{v}{s_0}$ tells us that $v$ contains a validation state
that reflects the server state $s_0$:
\[\exists((vs_0,cs_0)\in v)(asgn_0:\Var\to\Int),\satisfy{asgn_0} cs_0\wedge {vs_0}^{asgn_0}\equiv s_0\]

The corresponding validator step is constructed by analyzing the server step,
and proving small-step bisimulation for each derivation rule
in \autoref{sec:dualization}.

\paragraph{Write}
The server writes some expression $(e:\Sexp)$ to an address $!dst$.
According to \autoref{rule:write}, the validator creates a fresh variable $x_e$
for address $!dst$, and constraints that $(\#x_e\equiv e^{vs})$.\footnote{If
unspecified, $(vs,cs)$ represents the pre-small-step validator state, and $s$
represents the pre-small-step server state.}

We need to show that:
\begin{align*}
&\forall vs,cs,s,asgn,\\
&\satisfy{asgn}{cs}\wedge vs^{asgn}\equiv s\\
&\implies\forall d,e,\begin{array}[t]{lll}
\letin{s'&}{\update{s}{d}{e^s}&}\\
\letin{(vs',cs')&}{\Write(d,e,(vs,cs))&}\\
\multicolumn{3}{l}{\exists asgn',\quad\satisfy{asgn'}{cs'}\wedge vs'^{~asgn'}\equiv s'}
\end{array}
\end{align*}
\begin{proof}
Based on the definition of $\Write$, we need to show that:
\begin{align*}&\letin{x_e}{\Fresh(vs,cs)}\\
&\letin{vs'}{\update{vs}{d}{x_e}}\\
&\letin{cs'}{cs\cup\{x_e\equiv e^{vs}\}}\\
&\exists asgn',\quad\satisfy{asgn'}{cs'}\wedge vs'^{~asgn'}\equiv s'
\end{align*}
Let:\[asgn'=\update{asgn}{x_e}{e^{s}}\]

In order to prove $(\satisfy{asgn'}{cs'})$, we introduce some generic lemmas to
show that $(\satisfy{asgn'}{cs})$ and $({x_e}^{asgn'}\equiv{(e^{vs})^{asgn'}})$:
\begin{lemma}[Fresh variable preserves satisfaction]
\label{lem:fresh-sat}
\begin{align*}
&\forall (cs:\Set\constraint)(asgn:\Var\to\Int),\\
&\satisfy{asgn}{cs}\\
&\implies
\begin{array}[t]{lll}
\multicolumn{3}{l}{\forall (z:\Int),vs,}\\
\letin{x&}{\Fresh(vs,cs)&}\\
\letin{asgn'&}{\update{asgn}{x}{z}&}\\
\multicolumn{3}{l}{\satisfy{asgn'}{cs}}
\end{array}
\end{align*}
\begin{proof}
Since $x$ is fresh in $cs$, we have:
\[\forall (e_1\ccmp e_2)\in cs,\quad{e_1}^{asgn'}={e_1}^{asgn}\wedge{e_2}^{asgn'}={e_2}^{asgn}\]

Thus:
\begin{align*}
&\forall (e_1\ccmp e_2)\in cs,\quad{e_1}^{asgn'}\ccmp {e_2}^{asgn'}\\
&\textit{i.e. }\satisfy{asgn'} cs
\end{align*}
\end{proof}
\end{lemma}

\begin{lemma}[Fresh variable preserves evaluation]
\label{lem:fresh-eval}
\begin{align*}
&\forall (vs:\Nat\to\Var)(asgn:\Var\to\Int)(z:\Int),cs,\\
&\begin{array}[t]{lll}
\letin{x&}{\Fresh(vs,cs)&}\\
\letin{asgn'&}{\update{asgn}{x}{z}&}\\
\multicolumn{3}{l}{\forall (e:\Sexp),(e^{vs})^{asgn'}=(e^{vs})^{asgn}}
\end{array}
\end{align*}
\begin{proof}
Assume to the contrary that: \[(e^{vs})^{asgn'}\neq(e^{vs})^{asgn}\]

Since $asgn'$ is the same as $asgn$ except for variable $\#x$, we know that
$(e^{vs}:\Vexp)$ must involve $\#x$.  Therefore, $e$ must involve some address
$!k$ such that $(vs!k=x)$.  This contradicts the fact that $x$ is fresh in $vs$.
\end{proof}
\end{lemma}

\begin{lemma}[Symbolization preserves evaluation]
\label{lem:sym-eval}
\begin{align*}
&\forall(vs:\Nat\to\Var)(asgn:\Var\to\Int)(s:\Nat\to\Int),\\
&vs^{asgn}\equiv s\implies\forall (e:\Sexp),\quad(e^{vs})^{asgn}\equiv e^s
\end{align*}
\begin{proof}
Based on the definition of symbolization and evaluation:
\begin{itemize}
\item $e^{vs}$ substitutes all occurences of $!k$ in $e$ with $\#(vs!k)$;
\item $(e^{vs})^{asgn}$ substitutes all occurences of $\#(vs!k)$ to $asgn!(vs!k)$;
\item $e^s$ substitutes all occurences of $!k$ in $e$ with $(s!k)$.
\end{itemize}

From the hypothesis that $(vs^{asgn}\equiv s)$, we have:
\[\forall (k:\Nat),\quad asgn!(vs!k)\equiv (s!k)\]

Therefore, we know that all occurences of $!k$ were mapped to the same value
between the two evaluation paths.
\end{proof}
\end{lemma}

Based on \autoref{lem:fresh-eval}, we have:
\[{(e^{vs})}^{asgn'}={(e^{vs})}^{asgn}\]



Also, since $x_e$ is free in $vs$, and $asgn'$ is the same as $asgn$ except for
$x_e$, we have:
\[\forall k,asgn'!(vs'!k)=\begin{cases}
asgn'!x_e=e^s=(s'!k)&k\Is d\\
asgn!(vs!k)=(s!k)=(s'!k)&\text{otherwise}
\end{cases}\]
Therefore:\[vs'^{~asgn'}\equiv s'\]
\end{proof}

\paragraph{Havoc}
When the server writes some internal choice $c$ to address $d$,
according to \autoref{rule:choice}, the validator creates a fresh variable for
address $!d$.

We need to show that:
\begin{align*}&\forall vs,cs,s,asgn,\\
&\satisfy{asgn}{cs}\wedge vs^{asgn'}\equiv s\\
&\implies\forall d,c,\begin{array}[t]{lll}
\letin{s'&}{\update{s}{d}{c}&}\\
\letin{x_c&}{\Fresh(vs,cs)&}\\
\multicolumn{3}{l}{\exists asgn',\quad\satisfy{asgn'} cs\wedge vs^{asgn'}\equiv s'}
\end{array}
\end{align*}
\begin{proof}
Let:\[asgn'=\update{asgn}{x_c}{c}\]
Since $x_c$ is free in $cs$, we have
\end{proof}

%% \[\havoc(d,(vs,cs))=\letin{x_c}{\Fresh(vs,cs)}{(\update{vs}{d}{x_c},cs)}\]

%% \begin{proof}
%% We can construct the following assignment:
%% \[asgn_1=\update{asgn_0}{x_c}{c}\]


%% Since $x_c$ is also fresh in $vs_0$, we have:
%% \[\forall addr, asgn_1!(vs_1!addr)=\begin{cases}
%% asgn_1!x_c=c\equiv s_1!addr&addr\Is1\\
%% asgn_0!(vs_0!addr)=s_0!addr\equiv s_1!addr&\text{otherwise}
%% \end{cases}\]

%% Thus: \[{vs_1}^{asgn_1}\equiv s_1\]
%% \end{proof}

\section{Backward preservation lemma for rejection completeness}
\label{sec:rc2-proof}

\autoref{eq:rc2}
